rocq/demo/RecursiveFunctionReificationDemo.v
@@ -14,47 +14,27 @@ From impboot.demo Require Import DemoUtils.
 Fixpoint len (l: list nat): nat :=
   match l with
   | nil => 0%nat
-  | _ :: l1 => 1 + (len l1)
+  | _ :: l1 => 1 + len l1
   end.
 
 Theorem len_equation: ltac:(with_strategy opaque [Nat.add] ltac2:(unfold_fix_type '@len)).
 Proof. unfold_fix_proof '@len. Qed.
 
+Print len.
+
 Derive len_prog
   in ltac2:(relcompile_tpe 'len_prog 'len [])
   as len_prog_proof.
 Proof.
-  (* all: relcompile_start ().
-  all: relcompile_step ().
-  all: relcompile_step ().
-  all: relcompile_step ().
-  all: relcompile_step ().
-  Unshelve.
-  all: crush_side_conditions (); unfold name_enc in *; simpl in *; ltac1:(lia). *)
-
   relcompile_setup ().
-  revert l; ltac1:(fix IH 1).
-  intros.
-  rewrite len_equation.
+  revert l. ltac1:(fix IH 1); intros.
   eapply trans_app.
-  3: eauto.
-  2: reflexivity.
-  refine open_constr:(auto_list_case
-  (* env *) ltac2:(eauto)
-  (* s *) s
-  (* x0 x1 x2 *) _ _ _
-  (* name *) "h" "t"
-  (* v0 *) l
-  (* v1 *) 0%nat
-  (* v2 *) (fun _ t => (1 + (len t))%nat)
-  (* eval v0 *) _
-  (* eval v1 *) _
-  (* NoDup *) _
-  ).
-  1: typeclasses_eauto.
-  3,4,5,6: ltac1:(shelve).
-  1: eapply trans_Var.
-  1: unfold make_env; eauto with fenvDb.
+  3: eauto. 2: reflexivity.
+
+  rewrite len_equation.
+  eapply auto_list_case with (n1 := "h") (n2 := "t").
+  3: ltac1:(shelve).
+  1: eapply trans_Var; unfold make_env; eauto with fenvDb.
   destruct l.
   1: eapply auto_nat_const.
   eapply auto_nat_add.
@@ -65,3 +45,71 @@ Proof.
   Unshelve.
   all: crush_side_conditions (); unfold name_enc in *; simpl in *; ltac1:(lia).
 Qed.
+Print len_prog.
+
+(* all: relcompile_start ().
+  all: relcompile_step ().
+  all: relcompile_step ().
+  all: relcompile_step ().
+  all: relcompile_step ().
+  Unshelve.
+  all: crush_side_conditions (); unfold name_enc in *; simpl in *; ltac1:(lia). *)
+
+
+
+
+
+
+
+
+
+
+
+
+
+
+
+
+
+
+
+
+
+
+
+
+
+(* Fixpoint even (n: nat): bool :=
+  match n with
+  | 0%nat => true
+  | S n => negb (odd n)
+  end
+with odd (n: nat): bool :=
+  match n with
+  | 0%nat => false
+  | S n => negb (even n)
+  end.
+
+Theorem even_equation: ltac2:(unfold_fix_type '@even).
+Proof. unfold_fix_proof '@even. Qed.
+
+Theorem odd_equation: ltac2:(unfold_fix_type '@odd).
+Proof. unfold_fix_proof '@odd. Qed.
+
+Ltac2 Set relcompile_one_step := false.
+
+Derive even_prog
+  in ltac2:(relcompile_tpe 'even_prog 'even ['odd])
+  as even_prog_proof.
+Proof.
+  time relcompile.
+Qed.
+Print even_prog.
+
+Derive odd_prog
+  in ltac2:(relcompile_tpe 'odd_prog 'odd ['even])
+  as odd_prog_proof.
+Proof.
+  time relcompile.
+Qed.
+Print odd_prog. *)
