rocq/demo/BootstrappingIntuitionDemo.v
@@ -1,0 +1,28 @@
+From impboot Require Import Core.
+From coqutil Require Import Word.Interface Word.Properties.
+From impboot.imperative Require Import ImpSyntax.
+From impboot.functional Require Import FunValues.
+From impboot.imp2asm Require Import ImpToASMCodegen Compiler.
+Open Scope string.
+
+Locate compiler.
+
+Fail Compute (compiler compiler).
+
+About compiler.
+
+About codegen.
+
+Fail Compute (codegen compiler).
+
+Fail Definition compiler_magic: ImpSyntax.prog := compiler.
+
+Definition e (y: nat): nat :=
+  let x := 5 in
+  x + y.
+
+Definition e_imp: ImpSyntax.func :=
+  Func (name_enc "e") [name_enc "y"]
+    (Seq
+      (Assign (name_enc "x") (Const (word.of_Z 5)))
+      (Return (Add (Var (name_enc "x")) (Var (name_enc "y"))))).
