rocq/demo/Demo1.v
@@ -1,0 +1,20 @@
+From Stdlib Require Import Utf8 Lia.
+From Coq Require Import Extraction.
+
+From Corelib Require Import Byte.
+
+Definition e (x: nat) :=
+  let y := 3 in
+  x + y.
+
+Lemma e_correct: forall x,
+  3 <= e x.
+Proof.
+  intros; unfold e.
+  lia.
+Qed.
+
+Compute e 2.
+
+Extraction Language OCaml.
+Extraction "e.ml" e.
