rocq/demo/ExtractionDemo.v
@@ -1,0 +1,16 @@
+From Stdlib Require Import Utf8 Lia.
+From Coq Require Import Extraction.
+
+Definition e (y: nat): nat :=
+  let x := 5 in
+  x + y.
+
+Theorem e_correct: forall y, 5 ≤ e y.
+Proof.
+  intros; unfold e; lia.
+Qed.
+
+Compute e 3.
+
+Extraction Language OCaml.
+Extraction "e.ml" e.
